theories/Theorems/Spec.v
@@ -5,6 +5,7 @@ From Coq Require Import ZArith.BinInt.
 
 Require Import Utf8.Parser.
 Require Import Utf8.Spec.
+Require Import Utf8.Theorems.Enumerations.
 Require Import Utf8.Theorems.Order.
 
 Theorem valid_utf8_bytes_concat : forall (bytes1 bytes2: byte_str),
@@ -16,18 +17,6 @@ Proof.
   rewrite <- app_assoc. apply Utf8Concat. apply H. apply IHvalid_bytes1. apply valid_bytes2.
 Qed.
 
-Theorem valid_utf8_decompose : forall (bytes1 bytes2: byte_str),
-    valid_utf8_bytes (bytes1 ++ bytes2) ->
-    valid_utf8_bytes bytes1 ->
-    valid_utf8_bytes bytes2.
-Proof.
-  intros bytes1 bytes2 valid_concat valid_bytes1. induction valid_bytes1.
-  - assumption.
-  - rewrite <- app_assoc in valid_concat.
-    inversion valid_concat. symmetry in H1. apply app_eq_nil in H1. destruct H1. apply app_eq_nil in H1. destruct H1. subst. constructor.
-    Admitted.
-
-
 Lemma list_equals_self_append_implies_nil {T}: forall (list1 list2: list T),
     list1 = list1 ++ list2 ->
     list2 = nil.
@@ -36,25 +25,8 @@ Proof.
   destruct list1.
   - symmetry in H. apply List.app_eq_nil in H. destruct H. assumption. 
   - apply (f_equal (@length T)) in H.
-    rewrite List.length_app in H. simpl in H. Search (S (?a + ?b)). rewrite <- plus_Sn_m in H.
+    rewrite List.length_app in H. simpl in H. rewrite <- plus_Sn_m in H.
     destruct list2. reflexivity. simpl in H. lia.
-Qed.
-
-Lemma encoder_spec_implies_nil_mapsto_nil : forall encoder,
-    utf8_encoder_spec encoder ->
-    encoder nil = (nil, nil).
-Proof.
-  intros encoder encoder_spec_compliant.
-  assert (G := encoder_spec_compliant).
-  unfold utf8_encoder_spec, encoder_encode_correctly_implies_valid, encoder_encode_valid_codes_correctly, encoder_strictly_increasing, encoder_projects in G.
-  destruct G as [enc_implies_valid_utf8_bytes [valid_codepoints_iff_enc [enc_strictly_increasing enc_projects]]].
-  assert (valid_codepoints []) as nil_valid. apply Forall_nil.
-  apply valid_codepoints_iff_enc in nil_valid.
-  destruct nil_valid as [bytes encode_bytes].
-  specialize (enc_projects [] []). rewrite encode_bytes in enc_projects. simpl in enc_projects. rewrite enc_projects in encode_bytes. inversion encode_bytes.
-  symmetry in H0.
-  apply list_equals_self_append_implies_nil in H0.
-  subst. simpl in *. apply enc_projects.
 Qed.
 
 Lemma encoder_spec_injective : forall encoder,
@@ -65,11 +37,9 @@ Lemma encoder_spec_injective : forall encoder,
       codes1 = codes2.
 Proof.
   intros encoder encoder_spec_compliant.
-  assert (G := encoder_spec_compliant).
-  unfold utf8_encoder_spec, encoder_encode_correctly_implies_valid, encoder_encode_valid_codes_correctly, encoder_strictly_increasing, encoder_projects in G.
-  destruct G as [enc_implies_valid_utf8_bytes [valid_codepoints_iff_enc [enc_strictly_increasing enc_projects]]].
   intros codes1 codes2 bytes encoder_codes1 encoder_codes2.
-  specialize (enc_strictly_increasing codes1 codes2 bytes bytes encoder_codes1 encoder_codes2) as compare_codes.
+  destruct encoder_spec_compliant.
+  specialize (enc_increasing codes1 codes2 bytes bytes encoder_codes1 encoder_codes2) as compare_codes.
   unfold bytes_compare in compare_codes.
   rewrite list_compare_refl_if in compare_codes. 2: apply Z.compare_eq_iff.
   unfold codepoints_compare in compare_codes. apply list_compare_refl in compare_codes. apply compare_codes.
@@ -84,74 +54,223 @@ Lemma decoder_spec_injective : forall decoder,
       bytes1 = bytes2.
 Proof.
   intros decoder decoder_spec_compliant.
-  assert (G := decoder_spec_compliant).
-  unfold utf8_decoder_spec, decoder_decode_correctly_implies_valid, decoder_decode_valid_utf8_bytes_correctly, decoder_strictly_increasing in G.
-  destruct G as [dec_implies_valid_utf8_bytes [valid_bytes_iff_enc dec_strictly_increasing]].
+  destruct decoder_spec_compliant.
   intros bytes1 bytes2 codes decoder_bytes1 decoder_bytes2.
-  specialize (dec_strictly_increasing bytes1 bytes2 codes codes decoder_bytes1 decoder_bytes2) as compare_codes.
+  specialize (dec_increasing bytes1 bytes2 codes codes decoder_bytes1 decoder_bytes2) as compare_codes.
   unfold codepoints_compare in compare_codes.
   rewrite list_compare_refl_if in compare_codes. 2: apply Z.compare_eq_iff.
   unfold bytes_compare in compare_codes. symmetry in compare_codes. rewrite list_compare_refl in compare_codes.
   apply compare_codes. apply Z.compare_eq_iff.
 Qed.
 
-Lemma decoder_spec_projects_inverse: forall decoder,
+Theorem decoder_decode_valid_bytes : forall decoder,
     utf8_decoder_spec decoder ->
-    forall bytes codes1 codes2,
-      decoder bytes = (codes1 ++ codes2, []) ->
-      exists bytes1 bytes2,
-        decoder bytes1 = (codes1, []) /\
-          decoder bytes2 = (codes2, []) /\
-          bytes = bytes1 ++ bytes2.
-Admitted.
-
-Lemma decoder_spec_decode_app_valid_bytes : forall decoder,
-    utf8_decoder_spec decoder ->
-    forall bytes1 bytes2,
-      valid_utf8_bytes bytes1 ->
-      valid_utf8_bytes bytes2 ->
-      decoder (bytes1 ++ bytes2) =
-        let '(codes1, rest1) := decoder bytes1 in
-        let '(codes2, rest2) := decoder bytes2 in
-        (codes1 ++ codes2, []).
+    forall bytes,
+      valid_utf8_bytes bytes ->
+      exists codes, decoder bytes = (codes, []) /\ valid_codepoints codes.
 Proof.
-  intros decoder decoder_spec_compliant.
-  assert (G := decoder_spec_compliant).
-  unfold utf8_decoder_spec, decoder_decode_correctly_implies_valid, decoder_decode_valid_utf8_bytes_correctly, decoder_strictly_increasing in G.
-  destruct G as [dec_implies_valid_utf8_bytes [valid_bytes_iff_enc dec_strictly_increasing]].
-  Admitted.
-
-Lemma decoder_spec_nil_mapsto_nil : forall decoder,
-    utf8_decoder_spec decoder ->
-    decoder nil = (nil, []).
-  intros decoder decoder_spec_compliant.
-  assert (G := decoder_spec_compliant).
-  unfold utf8_decoder_spec, decoder_decode_correctly_implies_valid, decoder_decode_valid_utf8_bytes_correctly, decoder_strictly_increasing in G.
-  destruct G as [dec_implies_valid_utf8_bytes [valid_bytes_iff_dec dec_strictly_increasing]].
-  assert (valid_utf8_bytes []) as nil_valid. constructor. apply valid_bytes_iff_dec in nil_valid as G.
-  destruct G as [codes decode_codes].
-  assert (decode_codes_copy := decode_codes).
-  replace (nil) with (@nil Z ++ @nil Z) in decode_codes by reflexivity.
-  rewrite decoder_spec_decode_app_valid_bytes in decode_codes; try assumption.
-  rewrite decode_codes_copy in decode_codes.
-  inversion decode_codes. symmetry in H0.
-  apply list_equals_self_append_implies_nil in H0.
-  subst. assumption.
+  intros decoder decoder_spec.
+  intros bytes bytes_valid. induction bytes_valid.
+  - exists []. split. apply dec_nil. assumption. constructor.
+  - rewrite dec_projects; [| assumption].
+    apply (decoder_spec.(dec_input decoder)) in H.
+    destruct H as [code decode_bytes].
+    assert (exists code, decoder bytes = ([code], [])). exists code. assumption.
+    eapply dec_input in H; [| assumption].
+    eapply dec_output in H as code_valid; [| apply decoder_spec].
+    rewrite decode_bytes in code_valid.
+    destruct IHbytes_valid as [codes [decode_tail codes_valid]].
+    rewrite decode_bytes.
+    rewrite decode_tail.
+    exists ([code] ++ codes). split.
+    reflexivity.
+    apply Forall_cons; try assumption.
 Qed.
 
-Lemma encoder_spec_implies_nth_code_mapsto_nth_byte : forall encoder,
+Theorem encoder_encode_valid_codepoints : forall encoder,
     utf8_encoder_spec encoder ->
+    forall codes,
+      valid_codepoints codes ->
+      exists bytes, encoder codes = (bytes, []) /\ valid_utf8_bytes bytes.
+Proof.
+  intros encoder encoder_spec.
+  intros codes codes_valid. induction codes_valid as [| code tail].
+  - exists []. split. apply enc_nil. assumption. constructor.
+  - replace (code :: tail) with ([code] ++ tail) by reflexivity.
+    rewrite enc_projects; [| assumption].
+    apply (encoder_spec.(enc_input encoder)) in H.
+    destruct H as [bytes encode_code].
+    specialize (enc_output encoder encoder_spec code) as bytes_valid.
+    rewrite encode_code in bytes_valid.
+    destruct IHcodes_valid as [bytes_tail [encode_tail bytes_tail_valid]].
+    rewrite encode_code.
+    rewrite encode_tail.
+    exists (bytes ++ bytes_tail). split.
+    reflexivity.
+    apply Utf8Concat; try assumption.
+Qed.
+
+Definition encoder_to_option (encoder: encoder_type) code :=
+  match encoder [code] with
+  | (bytes, []) => Some bytes
+  | _ => None
+  end.
+
+Definition decoder_to_option (decoder: decoder_type) bytes :=
+  match decoder bytes with
+  | ([code], []) => Some code
+  | _ => None
+  end.
+
+Lemma encoder_partial_morphism : forall encoder,
+    utf8_encoder_spec encoder ->
+    partial_morphism valid_codepoint valid_codepoint_representation (encoder_to_option encoder).
+Proof.
+  intros encoder encoder_spec.
+  unfold encoder_to_option.
+  split.
+  - intros code bytes' encode_some.
+    destruct (encoder [code]) as [bytes rest] eqn:encoder_code.
+    destruct rest; [| discriminate].
+    specialize (enc_output encoder encoder_spec code) as bytes_valid.
+    rewrite encoder_code in bytes_valid.
+    inversion encode_some. subst.
+    apply bytes_valid.
+  - intros code encode_none code_valid.
+    destruct (encoder [code]) as [bytes rest] eqn: encoder_code.
+    destruct rest; [ discriminate|].
+    eapply enc_input in code_valid; [| apply encoder_spec].
+    destruct code_valid as [bytes' enc_code].
+    rewrite encoder_code in enc_code. inversion enc_code.
+Qed.
+
+   
+Lemma decoder_partial_morphism : forall decoder,
+    utf8_decoder_spec decoder ->
+    partial_morphism valid_codepoint_representation valid_codepoint (decoder_to_option decoder).
+Proof.
+  intros decoder decoder_spec.
+  unfold decoder_to_option.
+  assert (G := decoder_spec). destruct G.
+  split.
+  - intros bytes code bytes_some.
+    destruct (decoder bytes) as [codes rest] eqn:decode_bytes.
+    destruct codes as [| code2 tail]; [discriminate |].
+    destruct tail; [|discriminate].
+    destruct rest; [|discriminate].
+    inversion bytes_some. subst.
+    assert (exists code, decoder bytes = ([code], [])). exists code. assumption.
+    apply dec_input in H as bytes_valid.
+    specialize (dec_output bytes bytes_valid).
+    rewrite decode_bytes in dec_output.
+    assumption.
+  - intros bytes bytes_none bytes_valid.
+    destruct (decoder bytes) as [codes rest] eqn:decoder_bytes.
+    apply dec_input in bytes_valid.
+    destruct bytes_valid as [code decode_bytes].
+    rewrite decode_bytes in decoder_bytes.
+    destruct codes as [| code' tail].
+    + specialize (dec_nil) as enc_nil. unfold decoder_nil in enc_nil.
+      inversion decoder_bytes.
+    + destruct tail. destruct rest; [discriminate|].
+      all: inversion decoder_bytes.
+Qed.
+
+Lemma encoder_to_option_increasing : forall encoder,
+    utf8_encoder_spec encoder ->
+    increasing valid_codepoint Z.compare bytes_compare (encoder_to_option encoder).
+Proof.
+  intros encoder encoder_spec.
+  unfold encoder_to_option.
+  intros code1 code2 code1_valid code2_valid.
+  eapply enc_input in code1_valid; [| apply encoder_spec].
+  eapply enc_input in code2_valid; [| apply encoder_spec].
+  destruct code1_valid as [bytes1 encoder_code1].
+  destruct code2_valid as [bytes2 encoder_code2].
+  rewrite encoder_code1. rewrite encoder_code2.
+  specialize (enc_increasing encoder encoder_spec [code1] [code2] bytes1 bytes2 encoder_code1 encoder_code2) as increasing.
+  simpl in increasing.
+  destruct (code1 ?= code2); assumption.
+Qed.
+
+Lemma decoder_to_option_increasing: forall decoder,
+    utf8_decoder_spec decoder ->
+    increasing valid_codepoint_representation bytes_compare Z.compare (decoder_to_option decoder).
+Proof.
+  intros decoder decoder_spec.
+  unfold decoder_to_option.
+  intros bytes1 bytes2 bytes1_valid bytes2_valid.
+  eapply dec_input in bytes1_valid; [| apply decoder_spec].
+  eapply dec_input in bytes2_valid; [| apply decoder_spec].
+  destruct bytes1_valid as [code1 decoder_bytes1].
+  destruct bytes2_valid as [code2 decoder_bytes2].
+  rewrite decoder_bytes1, decoder_bytes2.
+  specialize (dec_increasing decoder decoder_spec bytes1 bytes2 [code1] [code2] decoder_bytes1 decoder_bytes2) as increasing.
+  simpl in increasing. symmetry in increasing.
+  destruct (code1 ?= code2); assumption.
+Qed.
+
+Lemma utf8_spec_implies_encoder_maps_nth_to_nth : forall encoder decoder,
+    utf8_encoder_spec encoder ->
+    utf8_decoder_spec decoder ->
     forall code bytes,
       encoder [code] = (bytes, []) -> 
       exists n, nth_valid_codepoint n = Some code /\ nth_valid_codepoint_representation n = Some bytes.
-Admitted.
+Proof.
+  intros encoder decoder encoder_spec decoder_spec code bytes encoder_code.
+  specialize (partial_isomorphism_countable_unique (0x10ffff - 0x7ff) valid_codepoint valid_codepoint_representation Z.compare bytes_compare) as iso.
+  specialize (iso inverse_nth_valid_codepoint inverse_nth_valid_codepoint_representation (decoder_to_option decoder)).
+  specialize (iso nth_valid_codepoint         nth_valid_codepoint_representation         (encoder_to_option encoder)).
+  specialize (iso codepoint_nth_isomorphism valid_codepoint_representation_isomorphism).
+  specialize (iso (encoder_partial_morphism encoder encoder_spec)).
+  specialize (iso (decoder_partial_morphism decoder decoder_spec)).
+  specialize (iso (encoder_to_option_increasing encoder encoder_spec)).
+  specialize (iso (decoder_to_option_increasing decoder decoder_spec)).
+  destruct iso as [going back].
+  unfold pointwise_equal in going.
+  assert (exists bytes, encoder [code] = (bytes, [])) as enc_bytes. exists bytes. assumption.
+  specialize (enc_input encoder encoder_spec code) as [G1 G2].
+  apply G2 in enc_bytes as code_valid.
+  specialize (going code code_valid).
+  unfold encoder_to_option in going.
+  rewrite encoder_code in going.
+  unfold and_then in going.
+  destruct (inverse_nth_valid_codepoint code) as [n|] eqn:inverse_nth_valid_codepoint; [|discriminate].
+  exists n. split.
+  - apply nth_valid_codepoint_invertible. split; assumption.
+  - symmetry in going. apply going.
+Qed.
 
-Lemma decoder_spec_implies_nth_bytes_mapsto_nth_code : forall decoder,
+Lemma utf8_spec_implies_decoder_maps_nth_to_nth : forall encoder decoder,
+    utf8_encoder_spec encoder ->
     utf8_decoder_spec decoder ->
-    forall bytes code,
+    forall code bytes,
       decoder bytes = ([code], []) -> 
-      exists n, nth_valid_codepoint n = Some code /\ nth_valid_byte n = Some bytes.
-Admitted.
+      exists n, nth_valid_codepoint n = Some code /\ nth_valid_codepoint_representation n = Some bytes.
+Proof.
+  intros encoder decoder encoder_spec decoder_spec code bytes decode_bytes.
+  specialize (partial_isomorphism_countable_unique (0x10ffff - 0x7ff) valid_codepoint valid_codepoint_representation Z.compare bytes_compare) as iso.
+  specialize (iso inverse_nth_valid_codepoint inverse_nth_valid_codepoint_representation (decoder_to_option decoder)).
+  specialize (iso nth_valid_codepoint         nth_valid_codepoint_representation         (encoder_to_option encoder)).
+  specialize (iso codepoint_nth_isomorphism valid_codepoint_representation_isomorphism).
+  specialize (iso (encoder_partial_morphism encoder encoder_spec)).
+  specialize (iso (decoder_partial_morphism decoder decoder_spec)).
+  specialize (iso (encoder_to_option_increasing encoder encoder_spec)).
+  specialize (iso (decoder_to_option_increasing decoder decoder_spec)).
+  destruct iso as [going back].
+  unfold pointwise_equal in back.
+  assert (exists code, decoder bytes = ([code], [])) as dec_code. exists code. assumption.
+  specialize (dec_input decoder decoder_spec bytes) as [G1 G2].
+  apply G2 in dec_code as bytes_valid.
+  specialize (back bytes bytes_valid).
+  unfold decoder_to_option in back.
+  rewrite decode_bytes in back.
+  unfold and_then in back.
+  destruct (inverse_nth_valid_codepoint_representation bytes) as [n|] eqn: inverse_nth_valid_codepoint_representation; [|discriminate].
+  exists n. split.
+  - symmetry. assumption.
+  - apply inverse_nth_valid_codepoint_representation_invertible; assumption.
+Qed.
 
 Theorem decode_encode_spec_inverses_for_single: forall encoder decoder,
     utf8_encoder_spec encoder ->
@@ -160,171 +279,126 @@ Theorem decode_encode_spec_inverses_for_single: forall encoder decoder,
       encoder [code] = (bytes, []) ->
       decoder bytes = ([code], []).
 Proof.
-  intros encoder decoder encoder_spec_compliant decoder_spec_compliant.
-  assert (G1 := encoder_spec_compliant).
-  assert (G2 := decoder_spec_compliant).
-  destruct G1 as [enc_implies_valid_utf8_bytes [valid_codepoints_iff_enc [enc_strictly_increasing enc_projects]]].
-  destruct G2 as [dec_implies_valid [valid_implies_dec dec_strictly_increasing]].
+  intros encoder decoder encoder_spec decoder_spec.
   intros code bytes encode_code.
-  apply enc_implies_valid_utf8_bytes in encode_code as G. destruct G as [bytes_valid _].
-  apply valid_implies_dec in bytes_valid as G. destruct G as [codes decode_bytes].
-  apply dec_implies_valid in decode_bytes as G. destruct G as [codes_valid _].
-  apply valid_codepoints_iff_enc in codes_valid as G. destruct G as [bytes2 encode_codes].
-  specialize (enc_strictly_increasing [code] codes bytes bytes2 encode_code encode_codes) as compare_code_codes.
-  specialize (encoder_spec_implies_nil_mapsto_nil encoder encoder_spec_compliant) as encode_nil.
-  specialize (decoder_spec_nil_mapsto_nil decoder decoder_spec_compliant) as decode_nil.
-  destruct codes as [|code2 codes_rest].
-  - specialize (decoder_spec_injective decoder decoder_spec_compliant [] bytes [] decode_nil decode_bytes) as G.
-    subst. simpl in compare_code_codes. destruct bytes2; discriminate.
-  - replace (code2 :: codes_rest) with ([code2] ++ codes_rest) in encode_codes, decode_bytes, codes_valid, compare_code_codes by reflexivity.
-    rewrite enc_projects in encode_codes.
-    destruct (encoder [code2]) as [bytes3 rest] eqn:encode_code2.
-    destruct (encoder codes_rest) as [bytes4 rest2] eqn:encode_codes_rest.
-    destruct rest; [|discriminate]. inversion encode_codes. subst. clear encode_codes.
-    specialize (enc_strictly_increasing [code] [code2] bytes bytes3 encode_code encode_code2) as compare_code_code2.
-    apply decoder_spec_projects_inverse in decode_bytes. 2: assumption.
-    destruct decode_bytes as [bytes1 [bytes2 [decode_bytes1 [decode_bytes2 bytes_eq]]]].
-    rewrite bytes_eq in compare_code_codes, compare_code_code2, encode_code, bytes_valid |- *.
-    destruct bytes1. rewrite decode_nil in decode_bytes1. inversion decode_bytes1.
-    rewrite <- app_comm_cons in bytes_valid.
-    destruct bytes3. specialize (encoder_spec_injective encoder encoder_spec_compliant [] [code2] [] encode_nil encode_code2) as G. inversion G.
-Admitted.
-    (* destruct_valid_bytes bytes_valid. *)
+  eapply utf8_spec_implies_encoder_maps_nth_to_nth in encode_code as G; [ | assumption | apply decoder_spec].
+  destruct G as [n [nth_code nth_byte]].
+  assert (exists bytes, encoder [code] = (bytes, [])) as code_valid. exists bytes. assumption.
+  apply enc_input in code_valid; [|assumption].
+  specialize (enc_output encoder encoder_spec code) as bytes_valid.
+  rewrite encode_code in bytes_valid.
+  eapply dec_input in bytes_valid; [| apply decoder_spec].
+  destruct bytes_valid as [code2 decode_code2].
+  eapply utf8_spec_implies_decoder_maps_nth_to_nth in decode_code2 as G; [ | apply encoder_spec | apply decoder_spec].
+  destruct G as [n2 [nth_code2 nth_byte2]].
+  apply nth_valid_codepoint_representation_invertible in nth_byte, nth_byte2.
+  rewrite nth_byte in nth_byte2. apply some_injective in nth_byte2.
+  subst. rewrite nth_code in nth_code2. apply some_injective in nth_code2. subst.
+  assumption.
+Qed.
 
-    
-   
 Theorem decode_encode_spec_compliant_decode_inverse_of_encode : forall encoder decoder,
     utf8_encoder_spec encoder ->
     utf8_decoder_spec decoder ->
-    forall (codes_big codes: list codepoint) bytes codes_suffix,
-      (length codes) <= (length codes_big) ->
+    forall codes bytes codes_suffix,
       encoder codes = (bytes, codes_suffix) ->
       exists codes_prefix, decoder bytes = (codes_prefix, nil) /\ codes = (codes_prefix ++ codes_suffix)%list.
 Proof.
-  intros encoder decoder encoder_spec_compliant decoder_spec_compliant.
-  assert (G1 := encoder_spec_compliant).
-  assert (G2 := decoder_spec_compliant).
-  unfold utf8_encoder_spec, encoder_encode_correctly_implies_valid, encoder_encode_valid_codes_correctly, encoder_strictly_increasing in G1.
-  destruct G1 as [enc_implies_valid_utf8_bytes [valid_codepoints_iff_enc [enc_strictly_increasing enc_projects]]].
-  unfold utf8_decoder_spec, decoder_decode_correctly_implies_valid, decoder_decode_valid_utf8_bytes_correctly, decoder_strictly_increasing in G2.
-  destruct G2 as [dec_implies_valid [valid_implies_dec dec_strictly_increasing]].
-  induction codes_big; intros codes bytes codes_suffix less_than encoder_codes.
-  - inversion less_than. apply length_zero_iff_nil in H0. subst.
-    specialize (encoder_spec_implies_nil_mapsto_nil encoder encoder_spec_compliant) as encode_nil.
-    rewrite encode_nil in encoder_codes. inversion encoder_codes. exists [].
-    split. apply decoder_spec_nil_mapsto_nil. apply decoder_spec_compliant. reflexivity.
-  - apply enc_implies_valid_utf8_bytes in encoder_codes as [bytes_valid [codes_prefix [codes_prefix_eq encoder_codes_prefix]]].
-    exists codes_prefix. destruct codes_prefix.
-    + rewrite encoder_spec_implies_nil_mapsto_nil in encoder_codes_prefix. 2: apply encoder_spec_compliant. inversion encoder_codes_prefix. split. apply decoder_spec_nil_mapsto_nil. apply decoder_spec_compliant. assumption.
-    + split; [| apply codes_prefix_eq].
-      replace (c :: codes_prefix) with ([c] ++ codes_prefix) in encoder_codes_prefix by reflexivity.
-      rewrite enc_projects in encoder_codes_prefix.
-      destruct (encoder [c]) as [bytes1 c_rest]  eqn:encoder_c.
-      destruct (encoder codes_prefix) as [bytes2 codes_rest] eqn:encoder_codes_prefix2.
-      destruct c_rest; try discriminate. inversion encoder_codes_prefix. subst.
-      rewrite length_app in less_than.
-      clear encoder_codes_prefix.
-      apply enc_implies_valid_utf8_bytes in encoder_c as G1, encoder_codes_prefix2 as G2.
-      destruct G1 as [bytes1_valid _]. destruct G2 as [bytes2_valid _].
-      simpl in less_than. apply IHcodes_big in encoder_codes_prefix2. 2: lia.
-      rewrite decoder_spec_decode_app_valid_bytes; try assumption.
-      destruct encoder_codes_prefix2 as [codes_prefix2 [decoder_bytes2 codes_prefix2_eq]]. subst.
-      rewrite decoder_bytes2. apply valid_implies_dec in bytes1_valid as [codes decode_bytes1].
-      rewrite decode_bytes1. rewrite app_nil_r.
-      rewrite pair_equal_spec. split; [| reflexivity].
-      replace (c :: codes_prefix2) with ([c] ++ codes_prefix2) by reflexivity.
-      clear decoder_bytes2. clear bytes2_valid.
-      apply app_inv_tail_iff.
-
-Theorem encoder_spec_implies_encode_single_equals : forall encoder1 code bytes,
+  intros encoder decoder encoder_spec decoder_spec.
+  induction codes as [| code tail]; intros bytes codes_suffix encode_codes.
+  - exists []. pose proof (enc_nil encoder encoder_spec). rewrite H in encode_codes. inversion encode_codes.
+    split. apply dec_nil. assumption. reflexivity.
+  - replace (code :: tail) with ([code] ++ tail) in encode_codes by reflexivity.
+    rewrite enc_projects in encode_codes; [| assumption].
+    destruct (encoder [code]) as [bytes2 rest] eqn:encoder_code.
+    destruct rest.
+    2: {
+      inversion encode_codes. subst.
+      specialize (enc_output encoder encoder_spec code) as bytes_invalid.
+      rewrite encoder_code in bytes_invalid. destruct bytes_invalid as [bytes_eq rest_eq].
+      inversion rest_eq. subst.
+      exists nil. split. apply dec_nil. assumption. reflexivity.
+    }
+    destruct (encoder tail) as [bytes3 rest] eqn:encoder_tail.
+    specialize (IHtail bytes3 rest ltac:(reflexivity)).
+    destruct IHtail as [codes_tail [decode_bytes3 tail_eq]].
+    inversion encode_codes.
+    rewrite dec_projects; [|assumption].
+    eapply decode_encode_spec_inverses_for_single in encoder_code; [ | assumption | apply decoder_spec].
+    rewrite encoder_code.
+    rewrite decode_bytes3.
+    exists ([code] ++ codes_tail). split. reflexivity. inversion tail_eq. subst. reflexivity.
+Qed.
+    
+Theorem encoder_spec_implies_encode_single_equals : forall encoder1 decoder code bytes,
     utf8_encoder_spec encoder1 ->
+    utf8_decoder_spec decoder ->
     encoder1 [code] = (bytes, nil) ->
     forall encoder2,
       utf8_encoder_spec encoder2 ->
       encoder2 [code] = (bytes, nil).
 Proof.
-  intros encoder1 code bytes encoder1_spec_compliant encoder1_code encoder2 encoder2_spec_compliant.
-  assert (G1 := encoder1_spec_compliant).
-  assert (G2 := encoder2_spec_compliant).
-  unfold utf8_encoder_spec, encoder_encode_correctly_implies_valid, encoder_encode_valid_codes_correctly, encoder_strictly_increasing, encoder_projects in G1, G2.
-  destruct G1 as [enc1_implies_valid_utf8_bytes [valid_codepoints_iff_enc1 [enc1_strictly_increasing enc1_projects]]].
-  destruct G2 as [enc2_implies_valid_utf8_bytes [valid_codepoints_iff_enc2 [enc2_strictly_increasing enc2_projects]]].
-  assert (exists bytes, encoder1 [code] = (bytes, nil)). exists bytes. assumption.
-  apply valid_codepoints_iff_enc1 in H.
-  apply valid_codepoints_iff_enc2 in H.
-  destruct H as [bytes2 encoder2_code]. rewrite encoder2_code.
-  apply pair_equal_spec. split; [| reflexivity].
-  Admitted.
-
+  intros encoder1 decoder code bytes encoder1_spec decoder_spec encoder1_code encoder2 encoder2_spec.
+  assert (exists bytes, encoder1 [code] = (bytes, [])) as valid_code. exists bytes. assumption.
+  eapply enc_input in valid_code; [| assumption].
+  eapply enc_input in valid_code; [| apply encoder2_spec].
+  destruct valid_code as [bytes2 encoder2_code].
+  eapply utf8_spec_implies_encoder_maps_nth_to_nth in encoder1_code as G1; [| assumption | apply decoder_spec].
+  eapply utf8_spec_implies_encoder_maps_nth_to_nth in encoder2_code as G2; [| assumption | apply decoder_spec].
+  destruct G1 as [n1 [nth1_code nth1_bytes]].
+  destruct G2 as [n2 [nth2_code nth2_bytes]].
+  apply nth_valid_codepoint_invertible in nth1_code, nth2_code.
+  destruct nth1_code as [inverse_n1 _], nth2_code as [inverse_n2 _].
+  rewrite inverse_n1 in inverse_n2. inversion inverse_n2. subst. rewrite nth1_bytes in nth2_bytes. inversion nth2_bytes. subst.
+  assumption.
+Qed.
    
-Theorem encoder_spec_implies_encoder_equal : forall encoder1 codes bytes,
+Theorem encoder_spec_implies_encoder_equal : forall encoder1 decoder codes bytes rest,
     utf8_encoder_spec encoder1 ->
-    encoder1 codes = (bytes, nil) ->
+    utf8_decoder_spec decoder ->
+    encoder1 codes = (bytes, rest) ->
     forall encoder2,
       utf8_encoder_spec encoder2 ->
-      encoder2 codes = (bytes, nil).
+      encoder2 codes = (bytes, rest).
 Proof.
-  intros encoder1.
-  induction codes as [| code codes_tail]; intros bytes encoder1_spec_compliant encoder1_codes encoder2 encoder2_spec_compliant; 
-    assert (G1 := encoder1_spec_compliant);
-    assert (G2 := encoder2_spec_compliant);
-    unfold utf8_encoder_spec, encoder_encode_correctly_implies_valid, encoder_encode_valid_codes_correctly, encoder_strictly_increasing, encoder_projects in G1, G2;
-    destruct G1 as [enc1_implies_valid_utf8_bytes [valid_codepoints_iff_enc1 [enc1_strictly_increasing enc1_projects]]];
-    destruct G2 as [enc2_implies_valid_utf8_bytes [valid_codepoints_iff_enc2 [enc2_strictly_increasing enc2_projects]]].
-  - specialize (enc1_projects nil nil) as enc_nil. simpl in enc_nil. rewrite encoder1_codes in enc_nil.
-    inversion enc_nil.
-    apply list_equals_self_append_implies_nil in H0. subst. clear enc_nil.
-    specialize (enc2_projects nil nil). simpl in enc2_projects.
-    destruct (encoder2 nil) as [bytes rest] eqn:E.
-    destruct rest.
-    + inversion enc2_projects. apply list_equals_self_append_implies_nil in H0. subst. reflexivity.
-    + apply enc2_implies_valid_utf8_bytes in E as G.
-      destruct G as [valid_utf8_bytes [codes_prefix [codes_eq enc_codes_prefix]]].
-      symmetry in codes_eq.
-      apply List.app_eq_nil in codes_eq as [codes_prefix_nil c_cons_rest_nil]. discriminate.
+  intros encoder1 decoder.
+  induction codes as [| code codes_tail]; intros bytes rest encoder1_spec decoder_spec encoder1_codes encoder2 encoder2_spec.
+  - pose proof (enc_nil encoder1 encoder1_spec) as encode1_nil. unfold encoder_nil in encode1_nil. rewrite encoder1_codes in encode1_nil.
+    inversion encode1_nil.
+    apply enc_nil. assumption.
   - replace (code :: codes_tail) with ([code] ++ codes_tail) in encoder1_codes |- * by reflexivity.
-    rewrite enc1_projects in encoder1_codes.
+    rewrite enc_projects in encoder1_codes; [| assumption].
     destruct (encoder1 [code]) as [bytes1 code_rest] eqn:encoder1_code.
     destruct code_rest; [|inversion encoder1_codes].
+    2: {
+      specialize (enc_output encoder1 encoder1_spec code) as G.
+      rewrite encoder1_code in G. destruct G. inversion H2. subst.
+      destruct (encoder2 [code]) as [bytes2 rest2] eqn:encoder2_code.
+      specialize (enc_output encoder2 encoder2_spec code) as G.
+      rewrite encoder2_code in G. destruct rest2.
+      + assert (exists bytes, encoder2 [code] = (bytes, [])) as code_valid. exists bytes2. assumption.
+        apply enc_input in code_valid; [|assumption].
+        eapply enc_input in code_valid; [|apply encoder1_spec].
+        destruct code_valid as [bytes encoder1_code2].
+        rewrite encoder1_code in encoder1_code2. inversion encoder1_code2.
+      + destruct G as [bytes_eq rest_eq]. inversion bytes_eq. inversion rest_eq. subst.
+        rewrite enc_projects; [|assumption].
+        rewrite encoder2_code. reflexivity.
+    } 
     destruct (encoder1 codes_tail) as [bytes2 codes_rest] eqn:encoder1_codes_tail.
     inversion encoder1_codes_tail. inversion encoder1_codes. subst.
-    specialize (IHcodes_tail bytes2 encoder1_spec_compliant ltac:(reflexivity) encoder2 encoder2_spec_compliant) as encoder2_codes_tail.
-    rewrite enc2_projects. rewrite encoder2_codes_tail.
+    specialize (IHcodes_tail bytes2 rest encoder1_spec decoder_spec ltac:(reflexivity) encoder2 encoder2_spec) as encoder2_codes_tail.
+    rewrite enc_projects. rewrite encoder2_codes_tail.
     assert (exists bytes, encoder1 [code] = (bytes, nil)). exists bytes1. assumption.
-    apply valid_codepoints_iff_enc1 in H.
-    apply valid_codepoints_iff_enc2 in H.
+    apply enc_input in H.
+    eapply enc_input in H; [| apply encoder2_spec].
     destruct H as [bytes3 encoder2_code]. rewrite encoder2_code.
     apply pair_equal_spec; split; auto.
     apply app_inv_tail_iff.
-    specialize (encoder_spec_implies_encode_single_equals encoder1 code bytes1 encoder1_spec_compliant encoder1_code encoder2 encoder2_spec_compliant) as G. rewrite G in encoder2_code. inversion encoder2_code.
+    specialize (encoder_spec_implies_encode_single_equals encoder1 decoder code bytes1 encoder1_spec decoder_spec encoder1_code encoder2 encoder2_spec) as G. rewrite G in encoder2_code. inversion encoder2_code.
     reflexivity.
+    all: assumption.
 Qed.
-
-(* Theorem encoder_spec_valid_all_equal : forall encoder decoder, *)
-(*     utf8_encoder_spec encoder -> *)
-(*     utf8_decoder_spec decoder -> *)
-(*     encoder nil = (nil, nil) /\ decoder nil = (nil, nil). *)
-(* Proof. *)
-(*   intros encoder decoder encoder_spec_compliant decoder_spec_compliant. *)
-(*   unfold utf8_encoder_spec, encoder_encode_correctly_implies_valid, encoder_encode_valid_codes_correctly, encoder_strictly_increasing in encoder_spec_compliant. *)
-(*   destruct encoder_spec_compliant as [enc_implies_valid_utf8_bytes [valid_codepoints_iff_enc enc_strictly_increasing]]. *)
-(*   unfold utf8_decoder_spec, decoder_decode_correctly_implies_valid, decoder_decode_valid_utf8_bytes_correctly, decoder_strictly_increasing in decoder_spec_compliant. *)
-(*   destruct decoder_spec_compliant as [dec_implies_valid [valid_implies_dec dec_strictly_increasing]]. *)
-(*   assert (valid_codepoints nil) as nil_valid_codepoints. { *)
-(*     apply List.Forall_nil. *)
-(*   } *)
-(*   apply valid_codepoints_iff_enc in nil_valid_codepoints as [bytes encode_nil]. *)
-(*   assert (valid_utf8_bytes nil) as nil_valid_bytes. { *)
-(*     constructor. *)
-(*   } *)
-(*   apply valid_implies_dec in nil_valid_bytes as [codes decode_nil]. *)
-(*   destruct (encoder codes) as [bytes2 codes_rest] eqn:encode_codes. *)
-(*   destruct (decoder bytes) as [codes2 bytes_rest] eqn:decode_bytes. *)
-(*   specialize (enc_strictly_increasing nil codes bytes bytes2 nil codes_rest encode_nil encode_codes). *)
-(*   specialize (dec_strictly_increasing nil bytes codes codes2 nil bytes_rest decode_nil decode_bytes). *)
-(*   unfold codepoints_lt in enc_strictly_increasing, dec_strictly_increasing. *)
-(*   simpl in enc_strictly_increasing, dec_strictly_increasing. *)
-(*   destruct codes. *)
 
 (* Theorem encoder_spec_valid_all_equal : forall encoder1 encoder2, *)
 (*     utf8_encoder_spec encoder1 -> *)
